---
title: Tutorial 9
updated: 2021-10-13T17:24:41.0000000+13:00
created: 2021-10-12T00:30:54.0000000+13:00
---

Tutorial 9
Monday, 11 October, 2021
7:30 PM

![image1](../../../../resources/e5822db566464eb79e731265bba2b01e.png)
1.)
1st girl: Sue
2nd girl: Cam
3rd girl: Ann

2.)
a%b = 0
a%c = 0

Therefore,
a%b+c = 0

a=bn,a=cn,n is an integerï¼Œbn=cn,so b%c=0,so b+c=kb,k is an integer,a=bn,,nb%kb=0,so a%(b+c)=0

3.)
<u>Definition:</u>
even + odd = odd
odd + odd = even
even + even = even

1.) 2xy will always be ==even==
even + ==even== + odd = odd
odd + ==even== + even = odd
even + even + even = even
odd + even + odd = even
From this we know either x and y must either be odd/even at the same time

In order for x - y to be odd, both x and y cannot be even/odd at the same time
So either x and y are odd or even. Which,
<u>Definition:</u>
odd - even = odd
even - odd = odd

4.) russel's paradox
5.)
![image2](../../../../resources/42d9efbe54c04d5bad2fe0e7275983cb.png)
![image3](../../../../resources/496fcbf204384de798ba9b65895460c8.png)
![image4](../../../../resources/fc4e7a2a6c424dec9bbb87379f0d19d0.png)
